

③ Using the definition of inner product

$$\langle a | b \rangle = \sum_{j=0}^{N-1} a_j \cdot b_j$$

$$\begin{aligned} \langle z^k | z^{k'} \rangle &= \sum_{j=0}^{N-1} (z_j^k) \cdot (z_j^{k'}) = \sum_{j=0}^{N-1} e^{-i2\pi k j / N} \cdot e^{i2\pi k' j / N} \\ &= \sum_{j=0}^{N-1} e^{i2\pi (k-k') j / N} \quad \textcircled{A} \end{aligned}$$

if $k' = k \rightarrow$ the exponent became 1, then the sum is N

if $k' \neq k$, and $r = e^{i2\pi (k'-k)/N}$ and S is the sum, then, equation \textcircled{A} become

$$S = 1 + r + r^2 + \dots + r^{N-1} \quad \textcircled{B}$$

multiplying by r on both sides

$$Sr = r + r^2 + r^3 + \dots + r^N \quad \textcircled{C}$$

Subtracting $\textcircled{B} - \textcircled{C}$ I obtain:

$$S - Sr = (1 + r + r^2 + \dots + r^{N-1}) - (r + r^2 + \dots + r^N)$$

$$S = \frac{1 - r^N}{1 - r} \rightarrow r^N = 1 \text{ because}$$

$$r^N = \left(e^{i2\pi (k'-k)/N} \right)^N = e^{i2\pi (k'-k)}$$

then I can say that

$S = 0$, then

$$\begin{aligned} e^{i2\pi m} &= \cos(2\pi m) + i \sin(2\pi m) \\ &= 1 + i \cdot 0 = 1 \end{aligned}$$

$$\frac{1}{N} \langle z^k | z^{k'} \rangle = \delta_{kk'}$$

$$r^N = 1$$

\Rightarrow orthogonal

④ $f(x) = \exp\left(-\frac{x^2}{2\sigma^2}\right)$

$$\bar{F}(q) = \int_{-\infty}^{\infty} f(x) e^{-iqx} dx$$

exponential:

$$-\frac{x^2}{2\sigma^2} - iqx = -\frac{1}{2\sigma^2} (x^2 + 2i\sigma^2 qx)$$

$$\rightarrow x^2 + 2i\sigma^2 qx = (x + i\sigma^2 q)^2 - (i\sigma^2 q)^2 = (x + i\sigma^2 q)^2 + \sigma^4 q^2$$

therefore

$$-\frac{x^2}{2\sigma^2} - iqx = -\frac{(x + i\sigma^2 q)^2}{2\sigma^2} - \frac{\sigma^4 q^2}{2}$$

I can do the transform

$$\bar{F}(q) = \int_{-\infty}^{\infty} \exp\left(-\frac{(x + i\sigma^2 q)^2}{2\sigma^2}\right) \exp\left(-\frac{\sigma^4 q^2}{2}\right) dx = e^{-\frac{\sigma^4 q^2}{2}} \underbrace{\int_{-\infty}^{\infty} \exp\left(-\frac{(x + i\sigma^2 q)^2}{2\sigma^2}\right) dx}_{\text{Gaussian integral, translated by } a = i\sigma^2 q}$$

\rightarrow the integral is a Gaussian integral, translated by $a = i\sigma^2 q$ and scaled by σ

$$\int_{-\infty}^{\infty} e^{-\frac{(x+a)^2}{2\sigma^2}} dx = \sigma \sqrt{2} \int_{-\infty}^{\infty} e^{-y^2} dy = \sigma \sqrt{2} \cdot \sqrt{\pi}$$

$$\bar{F}(q) = e^{-\sigma^4 q^2 / 2} \cdot \sqrt{2\pi} \cdot \sigma$$